### Properties of Matrix Addition

==========================Let A, B, C by========================== _==========================m x n==========================_ ==========================matrices and let 0 be the matrix whose entries are all 0’s.==========================

Then:

1. $A+B = B+A$﻿
2. $(A+B)+C = A+(B+C)$﻿
3. $A+0=A$﻿
4. There is a matrix $-A$﻿ such that: $A+(-A) = 0$﻿
    
    ==$-A$==﻿ ==is achieved by reversing the sign of all entries in== ==$A$==﻿
    

---

### Scalar Multiples

For a $m$﻿ x $n$﻿ matrix $A = [a_{ij}]$﻿ and scalar $K$﻿

$KA = [Ka_{ij}]$

---

### Properties of Scalar Multiples

For a $m$﻿ x $n $﻿ matrix $A $﻿ and $B$﻿ and scalars $r$﻿ and $s$﻿

1. $(r+s)A = rA + sA$﻿
2. $r(sA)=s(rA)=(rs)A$﻿
3. $rA=Ar$﻿
4. $r(A+B)=rA +rB$﻿

---

### Matrix Multiplication

For a $m$﻿ x $n$﻿ matrix $A$﻿ with columns $\vec{a_1}, \vec{a_2}, ... , \vec{a_n}$﻿, then we know

$ ⁍$

Suppose $A $﻿ is an $m$﻿ x $n$﻿ matrix and $B$﻿ is an $n$﻿ x $p$﻿ matrix.

Let the columns of $B$﻿ be $\vec{b_1}, \vec{b_2}, ..., \vec{b_p}$﻿.

Then $AB$﻿ is an $m$﻿ x $p$﻿ matrix whose columns are $A\vec{b_1}, A\vec{b_2}, ..., A\vec{b_p}$﻿ (in $\mathbb{R}^m$﻿)

==Example:==

$A = \begin{bmatrix}$﻿ (2x3)

$B = \begin{bmatrix}$﻿ (3x5)

$AB = \begin{bmatrix}$﻿  
  
$A\vec{b_1} = \begin{bmatrix}2&1&0\\5&3&-1\end{bmatrix}\begin{bmatrix}1\\0\\4\end{bmatrix}$﻿

$...$﻿

$A\vec{b_5} = \begin{bmatrix}2&1&0\\5&3&-1\end{bmatrix}\begin{bmatrix}-1\\1\\2\end{bmatrix}$﻿

so,

$AB = \begin{bmatrix}2&2&17&14&-1\\$﻿ (2x5)

> [!important]  
> @import url('https://cdnjs.cloudflare.com/ajax/libs/KaTeX/0.16.9/katex.min.css')ABAB AB﻿ has @import url('https://cdnjs.cloudflare.com/ajax/libs/KaTeX/0.16.9/katex.min.css')AAA﻿’s # of rows and @import url('https://cdnjs.cloudflare.com/ajax/libs/KaTeX/0.16.9/katex.min.css')BBB﻿’s # of columns  

---

### Properties of Matrix Multiplication

==Let== ==_A_== ==be an== ==_mxn_== ==matrix, and let== ==_B_== ==and== ==_C_== ==have sides for which the sums and products exist==

1. $A(BC) = (AB)C$﻿
2. $A(B+C) = AB + AC$﻿
3. $(B+C)A = BA + CA$﻿
4. $r(AB) = r(A)B = A(rB)$﻿
5. $I_mA = A = AI_m$﻿

(associative law of multiplication)

(left distributive law)

(right distributive law)

  

(identity for matrix multiplication)

---

### Identity Matrix

$I_1 = \begin {bmatrix} $﻿

$I_2 = \begin {bmatrix} 1 & 0 \\$﻿

$I_3 = \begin {bmatrix} $﻿

> [!important]  
> Note: matrix multiplication is not commutative. @import url('https://cdnjs.cloudflare.com/ajax/libs/KaTeX/0.16.9/katex.min.css')AB=ACAB = ACAB=AC﻿ but @import url('https://cdnjs.cloudflare.com/ajax/libs/KaTeX/0.16.9/katex.min.css')B≠CB \neq CB=C﻿  

---

### Row-Column Version of Matrix Multiplication

Dot product:

for $\vec{v_1} = \begin{bmatrix}\vec{v_1}\\\vec{v_2}\\...\\\vec{v_n}\end{bmatrix}$﻿ and $\vec{w} = \begin{bmatrix}\vec{w_1}\\\vec{w_2}\\...\\\vec{w_n}\end{bmatrix}$﻿ vectors in $\mathbb{R}^n$﻿

their ==dot product== is

$\vec{v}*\vec{w}=v_1w_1+v_2w_2+...+v_nw_n$﻿

Matrix $AB =$﻿

$\begin{bmatrix}$

$\begin{bmatrix}$

Example:

======$A = \begin{bmatrix}$======﻿ ======(2x3)======

==$B=\begin{bmatrix}$==﻿ ==(3x2)====$AB = \begin{bmatrix}$==﻿

> [!important]  
> Notice how @import url('https://cdnjs.cloudflare.com/ajax/libs/KaTeX/0.16.9/katex.min.css')ABABAB﻿ has @import url('https://cdnjs.cloudflare.com/ajax/libs/KaTeX/0.16.9/katex.min.css')AAA﻿’s # of rows and @import url('https://cdnjs.cloudflare.com/ajax/libs/KaTeX/0.16.9/katex.min.css')BBB﻿’s # of columns  

---

### The Transpose of a Matrix

Given an _m_ x _n_ matrix _$A$_﻿, the **transpose** of _$A$_﻿ is the _n_ x _m_ matrix, denoted by $A^T$﻿, whose columns are formed from the corresponding rows of _$A$_﻿_._

---

Example:

Let

$A = \begin {bmatrix}$

Then

$A^T = \begin {bmatrix}$

---

### Properties of a Transpose

Let $A$﻿ and $B$﻿ denote matrices whose sizes are appropriate for the following sums and products.

1. $(A^T)^T=A$﻿
2. $(A+B)^T=A^T+B^T$﻿
3. For any scalar $r$﻿, $(rA^T) = rA^T$﻿
4. $(AB)^T=B^TA^T$﻿

1. $(A^T)^T = A$﻿
2. $(A+B)^T = A^T + B^T$﻿
3. For any scalar $r$﻿, $(rA)^T = rA^T$﻿
4. $(AB)^T = B^T A^T $﻿

  

  

  

(Note, $C^T$﻿ is _p_ x _n_ and $A^T$﻿_n m)_